examples/low-level/crypto/Crypto.Symmetric.Poly1305.Spec.fst
@@ -204,7 +204,7 @@ let rec encode_bytes txt =
     SeqProperties.cons (encode w) (encode_bytes txt)
 
 
-#reset-options "--z3timeout 200"
+#reset-options "--z3timeout 1000"
 let rec lemma_encode_length txt: Lemma
   (ensures (Seq.length(encode_bytes txt) = (Seq.length txt + 15) / 16))
   (decreases (Seq.length txt))
@@ -422,6 +422,7 @@ let rec eq_poly p0 p1 =
   else if Seq.length p1 = 0 then eq_poly0 p0
   else SeqProperties.head p0 = SeqProperties.head p1 && eq_poly (SeqProperties.tail p0) (SeqProperties.tail p1)
 
+#reset-options "--z3timeout 1000"
 private let rec lemma_sane_eq_poly0 (p:seq elem) (r:elem) : Lemma
   (requires eq_poly0 p)
   (ensures (poly' p r = 0)) (decreases (Seq.length p)) = 
